fixed exists and immovable

refinedVST/typing/exist.v
@@ -2,28 +2,30 @@ From VST.typing Require Export type.
 From VST.typing Require Import programs optional.
 From VST.typing Require Import type_options.
 
-Definition ty_exists_rty_def `{!typeG Σ} {cs : compspecs} {A} (ty : A → type) (a : A) : type := ty a.
+Definition ty_exists_rty_def `{!typeG Ok_ty Σ} {cs : compspecs} {A} (ty : A → type) (a : A) : type := ty a.
 Definition ty_exists_rty_aux : seal (@ty_exists_rty_def). by eexists. Qed.
 Definition ty_exists_rty := (ty_exists_rty_aux).(unseal).
 Definition ty_exists_rty_eq : ty_exists_rty = @ty_exists_rty_def := (ty_exists_rty_aux).(seal_eq).
 Arguments ty_exists_rty {_ _ _} _ _.
 
 Section tyexist.
-  Context `{!typeG Σ} {cs : compspecs} {A : Type}.
+  Context `{!typeG Ok_ty Σ} {cs : compspecs} {A : Type}.
   (* rty has to be sealed as unification goes crazy otherwise (it will
   unify everything with tyexists). However rty_type must not use
   opaque as it cannot be unified with A otherwise by typeclass
   search. *)
-  Check ty_exists_rty.
   Program Definition tyexists_type (ty : A → type) (x : A) : type := {|
     ty_has_op_type := (ty x).(ty_has_op_type);
-    ty_own := (ty_exists_rty _ ty x).(ty_own); 
-    ty_own_val := (ty_exists_rty _ ty x).(ty_own_val); 
+    ty_own := (ty_exists_rty _ _ ty x).(ty_own); 
+    ty_own_val := (ty_exists_rty _ _ ty x).(ty_own_val); 
   |}.
   Next Obligation. move => *. rewrite ty_exists_rty_eq. by apply: ty_share. Qed.
   Next Obligation. move => *. rewrite ty_exists_rty_eq. by apply: ty_aligned. Qed.
-  Next Obligation. move => *. rewrite ty_exists_rty_eq. by eapply ty_deref. Qed.
-  Next Obligation. move => *. rewrite ty_exists_rty_eq. by apply: ty_ref. Qed.
+  Next Obligation. move => *. rewrite ty_exists_rty_eq. iIntros.
+                   iApply (ty_size_eq with "[$]"); try done. Qed.
+  Next Obligation. move => *. rewrite ! ty_exists_rty_eq. eapply ty_deref; eauto. Qed.
+  Next Obligation. move => *. rewrite ty_exists_rty_eq /ty_exists_rty_def.
+                   eapply ty_ref; eauto. Qed.
 
   Definition tyexists (ty : A → type) : rtype _ := RType (tyexists_type ty).
 
@@ -58,7 +60,7 @@ Notation "'∃ₜ' x .. y , p" := (ty_of_rty (tyexists (fun x => .. (ty_of_rty (
   : bi_scope.
 
 Section tyexist.
-  Context `{!typeG Σ} {cs : compspecs} {A : Type}.
+  Context `{!typeG Ok_ty Σ} {cs : compspecs} {A : Type}.
 
   Lemma simplify_hyp_place_tyexists x l β (ty : A → _) T:
     (l ◁ₗ{β} ty x -∗ T) ⊢ simplify_hyp (l◁ₗ{β} x @ tyexists ty) T.
